push intermediate work

src/Std/Data/DTreeMap/Slice.lean
@@ -16,53 +16,81 @@ public import Std.Data.DTreeMap
 namespace Std.DTreeMap
 open Std.Iterators
 
--- Zipper-based iterator for tree maps
-inductive MapIterator (α : Type u) (β : α → Type v) where
-  | done
-  | cons (k : α) (v : β k) (tree : Internal.Impl α β) (next : MapIterator α β)
+public def Internal.Impl.treeSize : Internal.Impl α β → Nat
+| .leaf => 0
+| .inner _ _ _ l r => 1 + l.treeSize + treeSize r
 
-def MapIterator.toList : MapIterator α β → List ((a : α) × β a)
+section MapIterator
+public inductive Zipper (α : Type u) (β : α → Type v) where
+  | done
+  | cons (k : α) (v : β k) (tree : Internal.Impl α β) (next : Zipper α β)
+
+variable {α : Type u} {β : α → Type v}
+
+public def Zipper.toList : Zipper α β → List ((a : α) × β a)
 | .done => []
 | .cons k v tree next => ⟨k,v⟩ :: tree.toList ++ next.toList
 
-def treeSize : Internal.Impl α β → Nat
-| .leaf => 0
-| .inner _ _ _ l r => 1 + treeSize l + treeSize r
+public def Zipper.keys : Zipper α β → List α
+| .done => []
+| .cons k _ tree next => k :: tree.keys ++ next.keys
 
-def MapIterator.size : MapIterator α β → Nat
+def Zipper.size : Zipper α β → Nat
 | .done => 0
-| .cons _ _ tree next => 1 + treeSize (tree) + next.size
+| .cons _ _ tree next => 1 + tree.treeSize + next.size
 
-def MapIterator.prependMap : Internal.Impl α β → MapIterator α β → MapIterator α β
+public def Zipper.WF [Ord α] : Zipper α β → Prop
+| .done => True
+| .cons k _ tree next => tree.keys.all (fun key => (compare key k).isLE) ∧ next.keys.all (fun key => (compare key k).isLE)
+
+public def Zipper.prependMap : Internal.Impl α β → Zipper α β → Zipper α β
   | .leaf, it => it
   | .inner _ k v l r, it => prependMap l (.cons k v r it)
 
-def prependMap_to_list (t : Internal.Impl α β) (it : MapIterator α β) : (MapIterator.prependMap t it).toList = t.toList ++ it.toList := by
+theorem prependMap_WF_inv [Ord α] [TransOrd α] {t : Internal.Impl α β} {wf : Internal.Impl.WF t} {z : Zipper α β} {z_wf : Zipper.WF z} : Zipper.WF (Zipper.prependMap t z) := by
+  induction t generalizing z
+  case leaf =>
+    simp [Zipper.prependMap]
+    exact z_wf
+  case inner _ k v l r l_ih r_ih =>
+    simp [Zipper.prependMap]
+    apply l_ih
+    . sorry
+    . constructor
+      sorry
+      sorry
+
+public theorem Zipper.prependMap_to_list (t : Internal.Impl α β) (it : Zipper α β) : (Zipper.prependMap t it).toList = t.toList ++ it.toList := by
   induction t generalizing it
   case leaf =>
-    simp [MapIterator.prependMap, Internal.Impl.toList_eq_toListModel]
+    simp [prependMap, Internal.Impl.toList_eq_toListModel]
   case inner _ k v l r l_ih r_ih =>
-    simp only [MapIterator.prependMap]
-    specialize l_ih (MapIterator.cons k v r it)
+    simp only [Zipper.prependMap]
+    specialize l_ih (Zipper.cons k v r it)
     rw [l_ih]
-    simp [MapIterator.toList, Internal.Impl.toList_eq_toListModel]
+    simp [toList, Internal.Impl.toList_eq_toListModel]
 
-variable (α : Type u) (β : α → Type v)
-theorem prependMap_size  (t : Internal.Impl α β) (it : MapIterator α β) : (MapIterator.prependMap t it).size = treeSize t + it.size := by
-  fun_induction MapIterator.prependMap
+theorem Zipper.prependMap_size (t : Internal.Impl α β) (it : Zipper α β) : (Zipper.prependMap t it).size = t.treeSize + it.size := by
+  fun_induction Zipper.prependMap
   case case1 =>
-   simp only [treeSize, Nat.zero_add]
+   simp only [Internal.Impl.treeSize, Nat.zero_add]
   case case2 size k v l r it ih =>
-    simp only [ih, MapIterator.size, treeSize, ← Nat.add_assoc, Nat.add_comm]
+    simp only [ih, Zipper.size, Internal.Impl.treeSize, ← Nat.add_assoc, Nat.add_comm]
 
-structure RxcIterator (cmp : α → α → Ordering) where
-  iter : MapIterator α β
+end MapIterator
+
+section Rxc
+
+public structure RxcIterator (α : Type u) (β : α → Type v) (cmp : α → α → Ordering) where
+  iter : Zipper α β
   upper : α
 
-def RxcIterator.inBounds {cmp : α → α → Ordering} (it : RxcIterator α β cmp) (k : α) : Bool :=
+variable {α : Type u} {β : α → Type v}
+
+public def RxcIterator.inBounds {cmp : α → α → Ordering} (it : RxcIterator α β cmp) (k : α) : Bool :=
   (cmp k it.upper).isLE
 
-def RxcIterator.step {cmp : α → α → Ordering} : RxcIterator α β cmp → IterStep (IterM (α := RxcIterator α β cmp) Id ((a : α) × β a)) ((a : α) × β a)
+public def RxcIterator.step {cmp : α → α → Ordering} : RxcIterator α β cmp → IterStep (IterM (α := RxcIterator α β cmp) Id ((a : α) × β a)) ((a : α) × β a)
   | ⟨.done, _⟩ => .done
   | ⟨.cons k v t it, upper⟩ =>
     if (cmp k upper).isLE then
@@ -70,11 +98,15 @@ def RxcIterator.step {cmp : α → α → Ordering} : RxcIterator α β cmp → 
     else
       .done
 
-instance : Iterator (RxcIterator α β cmp) Id ((a : α) × β a) where
+public instance : Iterator (RxcIterator α β cmp) Id ((a : α) × β a) where
   IsPlausibleStep it step := it.internalState.step = step
   step it := ⟨it.internalState.step, rfl⟩
 
-def RxC_finite : FinitenessRelation (RxcIterator α β cmp) Id where
+public instance : IteratorCollect (RxcIterator α β cmp) Id Id := .defaultImplementation
+
+public instance : IteratorCollectPartial (RxcIterator α β cmp) Id Id := .defaultImplementation
+
+def instFinitenessRelation : FinitenessRelation (RxcIterator α β cmp) Id where
   rel t' t := t'.internalState.iter.size < t.internalState.iter.size
   wf := by
     apply InvImage.wf
@@ -104,24 +136,197 @@ def RxC_finite : FinitenessRelation (RxcIterator α β cmp) Id where
           contradiction
         case isTrue heq =>
           simp at h'
-          simp only [h2, ← h'.1, prependMap_size, MapIterator.size, Nat.add_lt_add_iff_right,
+          simp only [h2, ← h'.1, Zipper.prependMap_size, Zipper.size, Nat.add_lt_add_iff_right,
             Nat.lt_add_left_iff_pos, Nat.lt_add_one]
 
-instance instFinite [TransCmp cmp] : Finite (RxcIterator α β cmp) Id :=
-  .of_finitenessRelation (RxC_finite α β)
+@[no_expose]
+public instance instFinite : Finite (RxcIterator α β cmp) Id :=
+  .of_finitenessRelation instFinitenessRelation
 
-instance : IteratorCollect (RxcIterator α β cmp) Id Id := .defaultImplementation
+public theorem toList_lemma {it : Iter (α := RxcIterator α β cmp) ((a : α) × β a)} : it.toList = it.internalState.iter.toList.filter (fun e => (cmp e.fst bound).isLE) := by
+  unfold Iter.toList
+  simp [Iter.toIterM]
+  unfold Iter.internalState
+  simp [instIteratorCollectRxcIteratorIdSigma]
+  sorry
 
-instance : IteratorCollectPartial (RxcIterator α β cmp) Id Id := .defaultImplementation
+public theorem step_rxcIterator_eq_match {cmp : α → α → Ordering} {it : IterM (α := RxcIterator α β cmp) Id ((a : α) × β a)} :
+    it.step = ⟨match it.internalState with
+    | { iter := Zipper.done, upper := _ } => IterStep.done
+    | { iter := Zipper.cons k v t it, upper := upper } =>
+      if (cmp k upper).isLE = true then
+        IterStep.yield { internalState := { iter := Zipper.prependMap t it, upper := upper } } ⟨k, v⟩
+      else IterStep.done,
+    (by simp only [IterM.IsPlausibleStep, Iterator.IsPlausibleStep, RxcIterator.step]; split; all_goals (rename_i heq; simp only [heq]))⟩ := by
+  simp [IterM.step, Iterator.step, RxcIterator.step]
+  ext
+  congr 1
 
-def test : Internal.Impl Nat fun _ => Nat :=
-  .ofList [⟨1, 2⟩, ⟨5, 4⟩, ⟨3, 1⟩, ⟨2, 8⟩, ⟨7, 9⟩, ⟨10, 5⟩]
+public structure RicSliceData (α : Type u) (β : α → Type v) (cmp : α → α → Ordering := by exact compare) where
+  treeMap : DTreeMap.Raw α β cmp
+  range : Ric α
 
-def iterLE (t : Internal.Impl α β) (comp : α → α → Ordering) (bound : α) : IterM (α := RxcIterator α β comp) Id ((a : α) × β a) :=
-  ⟨{iter := MapIterator.prependMap t .done, upper := bound }⟩
+public abbrev RicSlice α β cmp := Slice (RicSliceData α β cmp)
 
-#eval (iterLE _ _ test compare 5).allowNontermination.toList
+public instance : Ric.Sliceable (DTreeMap.Raw α β cmp) α (RicSlice α β cmp) where
+  mkSlice carrier range := ⟨carrier, range⟩
 
-section Rxc
+@[always_inline]
+public def RicSlice.Internal.iterM (s : RicSlice α β cmp) : IterM (α := RxcIterator α β cmp) Id ((a : α) × β a) :=
+  ⟨⟨Zipper.done.prependMap s.1.treeMap.inner, s.1.range.upper⟩⟩
+
+public instance {s : RicSlice α β cmp} : ToIterator s Id ((a : α) × β a) where
+  State := RxcIterator α β cmp
+  iterMInternal := RicSlice.Internal.iterM s
+
+def test : DTreeMap.Raw Nat (fun _ => Nat) compare := .ofList [⟨0, 0⟩, ⟨1, 1⟩, ⟨100, 3⟩, ⟨101, 4⟩]
+
+-- RxcIterator α β cmp
+public theorem step_iter_ricSlice_eq_match {α β} {cmp : α → α → Ordering} {t : DTreeMap.Raw α β cmp} {a b : α} :
+    t[*...=b].iter.step = ⟨match ({ iter := Zipper.prependMap t.inner Zipper.done, upper := b } : RxcIterator α β cmp) with
+        | { iter := Zipper.done, upper := upper } => IterStep.done
+        | { iter := Zipper.cons k v t it, upper := upper } =>
+          if (cmp k upper).isLE = true then
+            IterStep.yield { internalState := { iter := Zipper.prependMap t it, upper := upper } } ⟨k, v⟩
+          else IterStep.done, (sorry)⟩ := by
+  rw [Slice.iter_eq_toIteratorIter]
+  simp only [Ric.Sliceable.mkSlice, instSliceableRawRicSlice, RicSlice.Internal.iterM, ToIterator.iter_eq, IterM.toIter, Iter.step]
+  rw [step_rxcIterator_eq_match]
+  simp only [Iter.toIterM]
+  simp only [IterM.Step.toPure, IterStep.mapIterator, Id.run]
+  congr
+  split
+  case h_1 =>
+    rename_i heq
+    split at heq
+    any_goals contradiction
+    . rename_i heq2
+      simp at heq2
+      split at heq
+      . simp at heq
+        rename_i heq3
+        simp [heq3, ← heq.1, heq.2, IterM.toIter]
+      . contradiction
+  case h_2 =>
+    rename_i heq
+    split at heq
+    any_goals contradiction
+    . rename_i heq
+      split at heq
+      . contradiction
+      . contradiction
+  case h_3 =>
+    rename_i heq
+    split at heq
+    any_goals trivial
+    split at heq
+    . contradiction
+    . rename_i heq2
+      simp [heq2]
+
+public theorem toList_rocSlice_eq_filter_toList {α β} {cmp : α → α → Ordering}
+    {t : DTreeMap.Raw α β cmp} (h : t.WF) {bound : α} :
+    t[*...=bound].toList = t.toList.filter (fun e => (cmp e.fst bound).isLE) := by
+      simp only [Slice.toList_eq_toList_iter]
+      rw [Iter.toList_eq_match_step]
+      rw [step_iter_ricSlice_eq_match]
+      split
+      case h_1 x it' out heq =>
+        split at heq
+        any_goals contradiction
+        rename_i x' k v t it upper heq2
+        simp at heq2
+        split at heq
+        any_goals contradiction
+        simp at heq
+        rename_i isLE
+        rename_i t'
+        have ⟨heq₁, heq₂⟩ := heq
+        rw [← heq₂]
+        have := @Zipper.prependMap_to_list α β t'.inner .done
+        rw [heq2.1] at this
+        simp [Zipper.toList] at this
+        rw [← heq₁]
+        have toList_lemma := @toList_lemma α β cmp bound { internalState := { iter := Zipper.prependMap t it, upper := upper } }
+        simp at toList_lemma
+        rw [toList_lemma]
+        simp only [Raw.toList]
+        rw [← this]
+        simp only [List.filter, isLE, heq2.2]
+        congr
+        simp [Zipper.prependMap_to_list]
+      case h_2 =>
+        rename_i heq
+        split at heq
+        any_goals contradiction
+        . split at heq
+          any_goals contradiction
+      case h_3 x heq =>
+        split at heq
+        case h_1 it upper heq2 =>
+          simp at heq2
+          unfold Zipper.prependMap at heq2
+          split at heq2
+          . rename_i eq_empty
+            simp only [Raw.toList]
+            rw [eq_empty]
+            rw [Internal.Impl.toList_eq_toListModel]
+            simp only [Internal.Impl.toListModel_leaf, List.filter_nil]
+          . rename_i t₁ t₂ _ k v l r heq3
+            replace heq2 := heq2.1
+            sorry
+        case h_2 x' k v t it upper heq2 =>
+          split at heq
+          . contradiction
+          . rename_i t' notLE
+            simp at heq2
+            have ⟨heq2₁, heq2₂⟩ := heq2
+            clear heq2
+            have prependMap_to_List := @Zipper.prependMap_to_list α β t'.inner Zipper.done
+            simp [heq2₁, Zipper.toList] at prependMap_to_List
+            simp only [Raw.toList]
+            rw [← prependMap_to_List]
+            simp only [List.filter]
+            rw [← heq2₂] at notLE
+            simp only [notLE]
+
+            sorry
+      exact bound
+
+
+
+
+
+
+
+
+
+
+
+
+
+
+
+
+
+
+
+
+
+
+
+
+
+
+
+
+
+
+
+
+
+#eval test[*...=1].toList
+
+
 end Rxc
 end Std.DTreeMap
